add prove for mult

code/experimental/rsa/Multiplication.fst
@@ -10,34 +10,46 @@ module U64 = FStar.UInt64
 module U128 = FStar.UInt128
 open U32
 
-val mult_by_limb_addj:
+val mult_by_limb_addj_f:
+    a_i:U64.t -> l:U64.t -> c:U64.t -> r_ij:U64.t -> Tot (tuple2 U64.t U64.t)
+let mult_by_limb_addj_f a_i l c r_ij =
+    let res = U128.(mul_wide a_i l +^ uint64_to_uint128 c +^ uint64_to_uint128 r_ij) in
+    let r = U128.uint128_to_uint64 res in
+    let c' = U128.shift_right res 64ul in
+    let c' = U128.uint128_to_uint64 c' in
+    (c', r)
+
+val mult_by_limb_addj_:
     aLen:bnlen -> a:lbignum aLen ->
     l:U64.t -> i:U32.t{v i <= v aLen} -> j:U32.t ->
     resLen:U32.t{v aLen + v j < v resLen} ->
-    carry:U64.t -> res:lbignum resLen -> Stack unit
+    res:lbignum resLen -> Stack U64.t
     (requires (fun h -> live h a /\ live h res))
     (ensures  (fun h0 _ h1 -> live h0 a /\ live h0 res /\
         live h1 a /\ live h1 res /\ modifies_1 res h0 h1))
 
-let rec mult_by_limb_addj aLen a l i j resLen carry res =
-    if U32.(i <^ aLen) then begin
-        let res_ij = res.(i +^ j) in
-        let carry = U128.uint64_to_uint128 carry in
-        let res_ij = U128.uint64_to_uint128 res_ij in
+let rec mult_by_limb_addj_ aLen a l i j resLen res =
+    if i =^ 0ul then 0uL
+    else begin
+        let i1 = i -^ 1ul in
+        let c1 = mult_by_limb_addj_ aLen a l i1 j resLen res in
+        let (carry', res_ij) = mult_by_limb_addj_f a.(i1) l c1 res.(i1 +^ j) in
+        res.(i1 +^ j) <- res_ij;
+        carry'
+    end
 
-        let ai_l = U128.mul_wide a.(i) l in
-        let tmp = U128.add_mod ai_l carry in
-        let res_ij = U128.add_mod res_ij tmp in
+val mult_by_limb_addj:
+    aLen:bnlen -> a:lbignum aLen -> l:U64.t -> j:U32.t ->
+    resLen:U32.t{v aLen + v j < v resLen} ->
+    res:lbignum resLen -> Stack U64.t
+    (requires (fun h -> live h a /\ live h res))
+    (ensures  (fun h0 _ h1 -> live h0 a /\ live h0 res /\
+        live h1 a /\ live h1 res /\ modifies_1 res h0 h1))
 
-        let carry' = U128.shift_right res_ij 64ul in
-        let res_ij = U128.uint128_to_uint64 res_ij in
-        let carry' = U128.uint128_to_uint64 carry' in
-        res.(i +^ j) <- res_ij;
-        mult_by_limb_addj aLen a l (i +^ 1ul) j resLen carry' res end
-    else
-        res.(i +^ j) <- carry
+let mult_by_limb_addj aLen a l j resLen res =
+    mult_by_limb_addj_ aLen a l aLen j resLen res
 
-val mult_loop:
+val mult_:
     aLen:bnlen -> a:lbignum aLen ->
     bLen:bnlen -> b:lbignum bLen ->
     j:U32.t{U32.v j <= U32.v bLen} ->
@@ -46,11 +58,14 @@ val mult_loop:
     (ensures  (fun h0 _ h1 -> live h0 a /\ live h0 b /\ live h0 res /\
         live h1 a /\ live h1 b /\ live h1 res /\ modifies_1 res h0 h1))
 
-let rec mult_loop aLen a bLen b j resLen res =
-    if U32.(j <^ bLen) then begin
-        mult_by_limb_addj aLen a b.(j) 0ul j resLen 0uL res;
-        mult_loop aLen a bLen b (j +^ 1ul) resLen res
-        end
+let rec mult_ aLen a bLen b j resLen res =
+    if j =^ 0ul then ()
+    else begin
+        let j1 = j -^ 1ul in
+        mult_ aLen a bLen b j1 resLen res;
+        let c' = mult_by_limb_addj aLen a b.(j1) j1 resLen res in
+        res.(aLen +^ j1) <- c'
+    end
 
 (* res = a * b *)
 val mult:
@@ -62,7 +77,7 @@ val mult:
         live h1 a /\ live h1 b /\ live h1 res /\ modifies_1 res h0 h1))
         
 let mult aLen a bLen b res =
-    mult_loop aLen a bLen b 0ul (aLen +^ bLen) res
+    mult_ aLen a bLen b bLen (aLen +^ bLen) res
 
 (* TODO: res = a * a *)
 val sqr:
